@prefix : <https://ec.europa.eu/eurostat/NLP4StatRef/ontology/> .
@prefix owl: <http://www.w3.org/2002/07/owl#> .
@prefix rdf: <http://www.w3.org/1999/02/22-rdf-syntax-ns#> .
@prefix xml: <http://www.w3.org/XML/1998/namespace> .
@prefix xsd: <http://www.w3.org/2001/XMLSchema#> .
@prefix xsp: <http://www.owl-ontologies.com/2005/08/07/xsp.owl#> .
@prefix oecd: <https://ec.europa.eu/eurostat/NLP4StatRef/knowledge/oecd/> .
@prefix rdfs: <http://www.w3.org/2000/01/rdf-schema#> .
@prefix swrl: <http://www.w3.org/2003/11/swrl#> .
@prefix estat: <https://ec.europa.eu/eurostat/NLP4StatRef/ontology/> .
@prefix swrlb: <http://www.w3.org/2003/11/swrlb#> .
@prefix protege: <http://protege.stanford.edu/plugins/owl/protege#> .
@prefix estatdata: <https://ec.europa.eu/eurostat/NLP4StatRef/knowledge/> .
@base <https://ec.europa.eu/eurostat/NLP4StatRef/ontology/> .

<https://ec.europa.eu/eurostat/NLP4StatRef/ontology/> rdf:type owl:Ontology ;
                                                       rdfs:comment "This is the version 1.0 of the ontology for the NLP4StatRef Knowledge Database."@en ;
                                                       owl:versionInfo """2022.04.20 - This ontology carries all the classes and properties necessary for the description of the knowledge resulting from the processed data. 
It must be enriched with the description of the enrichments resulting from semantic analyses.
This version does not integrate the standard ontologies, the association being carried by the instantiation of the Knowledge database. An update of the ontology will be done, after the control of the instantiation, integrating then standard ontologies."""@en .

#################################################################
#    Object Properties
#################################################################

###  https://ec.europa.eu/eurostat/NLP4StatRef/ontology/hasCODEDTerm
estat:hasCODEDTerm rdf:type owl:ObjectProperty ;
                   rdfs:subPropertyOf estat:hasGlossaryTerm ;
                   rdfs:domain [ rdf:type owl:Class ;
                                 owl:unionOf ( estat:Classification
                                               estat:Content
                                             )
                               ] ;
                   rdfs:range estat:CODEDTerm ;
                   rdfs:comment "A property that relates entities from the Editorial Content or from Classification (Class, Category, etc.) with  CODED Terms"^^xsd:string ;
                   rdfs:label "hasCODEDTerm"^^xsd:string .


###  https://ec.europa.eu/eurostat/NLP4StatRef/ontology/hasCategory
estat:hasCategory rdf:type owl:ObjectProperty ;
                  rdfs:subPropertyOf estat:hasClassification ;
                  rdfs:domain estat:Content ;
                  rdfs:range estat:Category ;
                  rdfs:comment "A property that relates an article from the Editorial Content with its Categories"^^xsd:string ;
                  rdfs:label "hasCategory"^^xsd:string .


###  https://ec.europa.eu/eurostat/NLP4StatRef/ontology/hasCategoryOfGlossaryArticle
estat:hasCategoryOfGlossaryArticle rdf:type owl:ObjectProperty ;
                                   rdfs:subPropertyOf estat:hasCategory ;
                                   rdfs:domain estat:GlossaryArticle ;
                                   rdfs:range estat:GlossaryArticleCategory ;
                                   rdfs:comment "A property that relates an article from the glossary category with its category(-ies)"^^xsd:string ;
                                   rdfs:label "hasCategoryOfGlossaryArticle"^^xsd:string .


###  https://ec.europa.eu/eurostat/NLP4StatRef/ontology/hasCategoryOfStatisticExplainedArticle
estat:hasCategoryOfStatisticExplainedArticle rdf:type owl:ObjectProperty ;
                                             rdfs:subPropertyOf estat:hasCategory ;
                                             rdfs:domain estat:StatisticsExplainedArticle ;
                                             rdfs:range estat:StatisticsExplainedCategory ;
                                             rdfs:comment "A property that relates an article from the statistics explained category with its category(-ies)"^^xsd:string ;
                                             rdfs:label "hasCategoryOfStatisticExplainedArticle"^^xsd:string .


###  https://ec.europa.eu/eurostat/NLP4StatRef/ontology/hasClassification
estat:hasClassification rdf:type owl:ObjectProperty ;
                        rdfs:domain estat:Content ;
                        rdfs:range estat:Classification ;
                        rdfs:comment "A property that shows if an article from the Editorial Content has any Classification"^^xsd:string ;
                        rdfs:label "hasClassification"^^xsd:string .


###  https://ec.europa.eu/eurostat/NLP4StatRef/ontology/hasCode
estat:hasCode rdf:type owl:ObjectProperty ;
              rdfs:subPropertyOf estat:hasGlossaryTerm ;
              rdfs:domain estat:StatisticalData ;
              rdfs:range estat:Code ;
              rdfs:comment "A property that relates a dataset to its code(-s). Basically is the labels of the Statistical Data"^^xsd:string ;
              rdfs:label "hasCode"^^xsd:string .


###  https://ec.europa.eu/eurostat/NLP4StatRef/ontology/hasFrequentTerm
estat:hasFrequentTerm rdf:type owl:ObjectProperty ;
                      rdfs:subPropertyOf estat:hasGlossaryTerm ;
                      rdfs:domain estat:Topic ;
                      rdfs:range estat:FrequentTerm ;
                      rdfs:comment "A property that relates a Topic (from Quanto's Topic Modelling) with the frequently used terms that it contains"^^xsd:string ;
                      rdfs:label "hasFrequentTerm"^^xsd:string .


###  https://ec.europa.eu/eurostat/NLP4StatRef/ontology/hasGlossaryTerm
estat:hasGlossaryTerm rdf:type owl:ObjectProperty ;
                      rdfs:domain [ rdf:type owl:Class ;
                                    owl:unionOf ( estat:Classification
                                                  estat:Content
                                                )
                                  ] ;
                      rdfs:range estat:GlossaryTerm ;
                      rdfs:comment "A property that shows if an article from the Editorial Content has any Glossary Term"^^xsd:string ;
                      rdfs:label "hasGlossaryTerm"^^xsd:string .


###  https://ec.europa.eu/eurostat/NLP4StatRef/ontology/hasOECDTerm
estat:hasOECDTerm rdf:type owl:ObjectProperty ;
                  rdfs:subPropertyOf estat:hasGlossaryTerm ;
                  rdfs:domain [ rdf:type owl:Class ;
                                owl:unionOf ( estat:Classification
                                              estat:Content
                                            )
                              ] ;
                  rdfs:range estat:OECDTerm ;
                  rdfs:comment "A property that relates entities from the Editorial Content or from a Classification (Class, Category, etc.) with  OECD Terms"^^xsd:string ;
                  rdfs:label "hasOECDTerm" .


###  https://ec.europa.eu/eurostat/NLP4StatRef/ontology/hasOECDTheme
estat:hasOECDTheme rdf:type owl:ObjectProperty ;
                   rdfs:subPropertyOf estat:hasTheme ;
                   rdfs:domain estat:OECDTerm ;
                   rdfs:range estat:OECDTheme ;
                   rdfs:comment "A property that relates the OECD themes with the OECD terms"^^xsd:string ;
                   rdfs:label "hasOECDTheme"^^xsd:string .


###  https://ec.europa.eu/eurostat/NLP4StatRef/ontology/hasParagraph
estat:hasParagraph rdf:type owl:ObjectProperty ;
                   rdfs:domain estat:StatisticsExplainedArticle ;
                   rdfs:range estat:Paragraph ;
                   rdfs:comment "A property that relates the Statistics Explained Articles with its paragraphs"^^xsd:string ;
                   rdfs:label "hasParagraph"^^xsd:string .


###  https://ec.europa.eu/eurostat/NLP4StatRef/ontology/hasReference
estat:hasReference rdf:type owl:ObjectProperty ;
                   rdfs:domain [ rdf:type owl:Class ;
                                 owl:unionOf ( estat:Content
                                               estat:GlossaryTerm
                                             )
                               ] ;
                   rdfs:range estat:Reference ;
                   rdfs:comment "A property that relates an article or a dataset with its resources" ;
                   rdfs:label "hasResource" .


###  https://ec.europa.eu/eurostat/NLP4StatRef/ontology/hasSubTheme
estat:hasSubTheme rdf:type owl:ObjectProperty ;
                  rdfs:domain estat:EurostatTheme ;
                  rdfs:range estat:EurostatTheme .


###  https://ec.europa.eu/eurostat/NLP4StatRef/ontology/hasTheme
estat:hasTheme rdf:type owl:ObjectProperty ;
               rdfs:subPropertyOf estat:hasClassification ;
               rdfs:domain estat:Content ;
               rdfs:range estat:Theme ;
               rdfs:label "hasTheme"^^xsd:string ;
               owl:backwardCompatibleWith "A property that relates the Editorial Content entities with their Theme(-s)"^^xsd:string .


###  https://ec.europa.eu/eurostat/NLP4StatRef/ontology/hasTopic
estat:hasTopic rdf:type owl:ObjectProperty ;
               rdfs:subPropertyOf estat:hasClassification ;
               rdfs:domain estat:Content ;
               rdfs:range estat:Topic ;
               rdfs:comment "A property that relates an article from the Editorial Content with its Topics"^^xsd:string ;
               rdfs:label "hasTopic"^^xsd:string .


###  https://ec.europa.eu/eurostat/NLP4StatRef/ontology/hasType
estat:hasType rdf:type owl:ObjectProperty ;
              rdfs:subPropertyOf estat:hasClassification ;
              rdfs:domain estat:Content ;
              rdfs:range estat:Type ;
              rdfs:comment "Some articles from the Editorial Content may have some information about their lexical type, status type, and others"^^xsd:string ;
              rdfs:label "hasType"^^xsd:string .


###  https://ec.europa.eu/eurostat/NLP4StatRef/ontology/hasURI
estat:hasURI rdf:type owl:ObjectProperty ;
             rdfs:domain estat:Reference ;
             rdfs:range estat:Content ;
             rdfs:comment "A property that relates referenced resources with an entity from the content class" ;
             rdfs:label "hasURI" .


###  https://ec.europa.eu/eurostat/NLP4StatRef/ontology/relatedTerm
estat:relatedTerm rdf:type owl:ObjectProperty ;
                  rdfs:domain estat:GlossaryTerm ;
                  rdfs:range estat:GlossaryTerm ;
                  rdfs:comment "A property that relaetes glossary terms to another glossary term" .


###  https://ec.europa.eu/eurostat/NLP4StatRef/ontology/relatedTheme
estat:relatedTheme rdf:type owl:ObjectProperty ;
                   rdfs:subPropertyOf owl:topObjectProperty ;
                   rdfs:domain estat:EurostatTheme ;
                   rdfs:range estat:OECDTheme ;
                   rdfs:comment "A property that relates a OECD Entity with the EuroStat Theme(-s)"^^xsd:string ;
                   rdfs:label "MapsToTheme"^^xsd:string .


#################################################################
#    Data properties
#################################################################

###  https://ec.europa.eu/eurostat/NLP4StatRef/ontology/content
estat:content rdf:type owl:DatatypeProperty ;
              rdfs:domain estat:Article ;
              rdfs:range xsd:string ;
              rdfs:comment "This property relates the articles from the editorial content with their Content (i.e., their Abstract or a small Description)"^^xsd:string ;
              rdfs:label "content"^^xsd:string .


###  https://ec.europa.eu/eurostat/NLP4StatRef/ontology/context
estat:context rdf:type owl:DatatypeProperty ;
              rdfs:domain [ rdf:type owl:Class ;
                            owl:unionOf ( estat:Article
                                          estat:OECDTerm
                                        )
                          ] ;
              rdfs:range xsd:string ;
              rdfs:comment "A property that relates the Articles from the Editorial Content with their context (a small description of the context that the article is applicable to)"^^xsd:string ;
              rdfs:label "context"^^xsd:string .


###  https://ec.europa.eu/eurostat/NLP4StatRef/ontology/dataSource
estat:dataSource rdf:type owl:DatatypeProperty ;
                 rdfs:domain estat:Article ;
                 rdfs:range xsd:string ;
                 rdfs:comment "A property that connects the articles from the Editorial Content with their Data Source(-s)"^^xsd:string ;
                 rdfs:label "dataSource"^^xsd:string .


###  https://ec.europa.eu/eurostat/NLP4StatRef/ontology/dateCreated
estat:dateCreated rdf:type owl:DatatypeProperty ;
                  rdfs:domain [ rdf:type owl:Class ;
                                owl:unionOf ( estat:Content
                                              estat:GlossaryTerm
                                            )
                              ] ;
                  rdfs:range xsd:dateTimeStamp ;
                  rdfs:comment "A property that relates a glossary entity with its creation date"^^xsd:string ;
                  rdfs:label "dateCreated"^^xsd:string .


###  https://ec.europa.eu/eurostat/NLP4StatRef/ontology/dateUpdated
estat:dateUpdated rdf:type owl:DatatypeProperty ;
                  rdfs:domain [ rdf:type owl:Class ;
                                owl:unionOf ( estat:Content
                                              estat:GlossaryTerm
                                            )
                              ] ;
                  rdfs:range xsd:dateTimeStamp ;
                  rdfs:comment "A property that relates a glossary entity with the date that was updated"^^xsd:string ;
                  rdfs:label "dateUpdated"^^xsd:string .


###  https://ec.europa.eu/eurostat/NLP4StatRef/ontology/definition
estat:definition rdf:type owl:DatatypeProperty ;
                 rdfs:domain [ rdf:type owl:Class ;
                               owl:unionOf ( estat:CODEDTerm
                                             estat:OECDTerm
                                           )
                             ] ;
                 rdfs:range xsd:string ;
                 rdfs:comment "A property that relates a glossary entity with its context"^^xsd:string ;
                 rdfs:label "definition"^^xsd:string .


###  https://ec.europa.eu/eurostat/NLP4StatRef/ontology/fileDescription
estat:fileDescription rdf:type owl:DatatypeProperty ;
                      rdfs:domain estat:StatisticalData ;
                      rdfs:range xsd:string ;
                      rdfs:comment "A property that relates a dataset with its file description"^^xsd:string ;
                      rdfs:label "fileDescription"^^xsd:string .


###  https://ec.europa.eu/eurostat/NLP4StatRef/ontology/fileLink
estat:fileLink rdf:type owl:DatatypeProperty ;
               rdfs:domain estat:StatisticalData ;
               rdfs:range xsd:anyURI ;
               rdfs:comment "A property that indicates the link of a dataset" ;
               rdfs:label "fileLink" .


###  https://ec.europa.eu/eurostat/NLP4StatRef/ontology/hasURL
estat:hasURL rdf:type owl:DatatypeProperty ;
             rdfs:range xsd:anyURI ;
             rdfs:comment "A property that contains the URL(s) of any resource"^^xsd:string ;
             rdfs:label "hasURL"^^xsd:string .


###  https://ec.europa.eu/eurostat/NLP4StatRef/ontology/id
estat:id rdf:type owl:DatatypeProperty ;
         rdfs:domain [ rdf:type owl:Class ;
                       owl:unionOf ( estat:Content
                                     estat:GlossaryTerm
                                   )
                     ] ;
         rdfs:range xsd:integer ;
         rdfs:comment "A property that indicates the ID of the glossary or the content entity"^^xsd:string ;
         rdfs:label "id"^^xsd:string .


###  https://ec.europa.eu/eurostat/NLP4StatRef/ontology/keyword
estat:keyword rdf:type owl:DatatypeProperty ;
              rdfs:domain estat:Topic ;
              rdfs:range xsd:string ;
              rdfs:label "A property that relates the an instance from the class Topic with its keyword(-s)"^^xsd:string ,
                         "keyword"^^xsd:string .


###  https://ec.europa.eu/eurostat/NLP4StatRef/ontology/level
estat:level rdf:type owl:DatatypeProperty ;
            rdfs:domain estat:StatisticalData ;
            rdfs:range xsd:string ;
            rdfs:comment "A property that indicates the depth that the dataset is in the Statistical Data tree"^^xsd:string ;
            rdfs:label "level"^^xsd:string .


###  https://ec.europa.eu/eurostat/NLP4StatRef/ontology/linkID
estat:linkID rdf:type owl:DatatypeProperty ;
             rdfs:domain estat:Reference ;
             rdfs:range xsd:integer ;
             rdfs:comment "A property that indicates the ID of the link. The ID is given by EuroStat"^^xsd:string ;
             rdfs:label "linkID"^^xsd:string .


###  https://ec.europa.eu/eurostat/NLP4StatRef/ontology/paragraph
estat:paragraph rdf:type owl:DatatypeProperty ;
                rdfs:domain estat:Paragraph ;
                rdfs:range xsd:string ;
                rdfs:comment "A property that relates a paragraph from the paragraph class with its context"^^xsd:string ;
                rdfs:label "paragraph"^^xsd:string .


###  https://ec.europa.eu/eurostat/NLP4StatRef/ontology/remark
estat:remark rdf:type owl:DatatypeProperty ;
             rdfs:domain estat:CODEDTerm ;
             rdfs:range xsd:string ;
             rdfs:comment "A property that relates a glossary entity with its remark"^^xsd:string ;
             rdfs:label "remark"^^xsd:string .


###  https://ec.europa.eu/eurostat/NLP4StatRef/ontology/sourcePublication
estat:sourcePublication rdf:type owl:DatatypeProperty ;
                        rdfs:domain estat:OECDTerm ;
                        rdfs:range xsd:string ;
                        rdfs:comment "A property that relates the OECD enities with their source Publication"^^xsd:string ;
                        rdfs:label "sourcePublication"^^xsd:string .


###  https://ec.europa.eu/eurostat/NLP4StatRef/ontology/term
estat:term rdf:type owl:DatatypeProperty ;
           rdfs:domain estat:GlossaryTerm ;
           rdfs:range xsd:string ;
           rdfs:comment "A property that indicates the label of the dataset and the label of the Vocabulary entity"^^xsd:string ;
           rdfs:label "term"^^xsd:string .


###  https://ec.europa.eu/eurostat/NLP4StatRef/ontology/title
estat:title rdf:type owl:DatatypeProperty ;
            rdfs:range xsd:string ;
            rdfs:comment "This property relates the articles from the editorial content with their Title"^^xsd:string ;
            rdfs:label "title"^^xsd:string .


#################################################################
#    Classes
#################################################################

###  https://ec.europa.eu/eurostat/NLP4StatRef/ontology/Article
estat:Article rdf:type owl:Class ;
              rdfs:subClassOf estat:Content ;
              rdfs:comment "All the information written and published around the statistical data, to comment on them and explain them."@en ;
              rdfs:label "Article"@en .


###  https://ec.europa.eu/eurostat/NLP4StatRef/ontology/BackgroundArticle
estat:BackgroundArticle rdf:type owl:Class ;
                        rdfs:subClassOf estat:StatisticsExplainedArticle ;
                        rdfs:comment "A class with the Statistics Explained Articles that are also Background Articles"^^xsd:string ;
                        rdfs:label "Background Article"^^xsd:string .


###  https://ec.europa.eu/eurostat/NLP4StatRef/ontology/CODEDTerm
estat:CODEDTerm rdf:type owl:Class ;
                rdfs:subClassOf estat:GlossaryTerm ;
                rdfs:comment "Glossary is an alphabetical list of terms relating to a specific subject enriched by definitions and related content."@en ;
                rdfs:label "CODEDTerm"@en .


###  https://ec.europa.eu/eurostat/NLP4StatRef/ontology/Category
estat:Category rdf:type owl:Class ;
               rdfs:subClassOf estat:Classification ;
               rdfs:label "A class that represent the Categories that EuroStat offers"^^xsd:string ,
                          "Category"^^xsd:string .


###  https://ec.europa.eu/eurostat/NLP4StatRef/ontology/Classification
estat:Classification rdf:type owl:Class ;
                     rdfs:comment "All types of controlled Category, Types, Topics, and others"^^xsd:string ;
                     rdfs:label "Classification"^^xsd:string .


###  https://ec.europa.eu/eurostat/NLP4StatRef/ontology/Code
estat:Code rdf:type owl:Class ;
           rdfs:subClassOf estat:GlossaryTerm ;
           rdfs:comment "A class that contains the codes that the statistical datasets are related to"^^xsd:string ;
           rdfs:label "Code"^^xsd:string .


###  https://ec.europa.eu/eurostat/NLP4StatRef/ontology/ConceptType
estat:ConceptType rdf:type owl:Class ;
                  rdfs:subClassOf estat:Type ;
                  rdfs:comment "A class with the concept types"^^xsd:string ;
                  rdfs:label "ConceptType"^^xsd:string .


###  https://ec.europa.eu/eurostat/NLP4StatRef/ontology/Content
estat:Content rdf:type owl:Class ;
              rdfs:comment "All types of described and annotated content."@en ;
              rdfs:label "Content"@en .


###  https://ec.europa.eu/eurostat/NLP4StatRef/ontology/Database
estat:Database rdf:type owl:Class ;
               rdfs:subClassOf estat:SEAReference ;
               rdfs:comment "A class with the resources of the database" ;
               rdfs:label "Database" .


###  https://ec.europa.eu/eurostat/NLP4StatRef/ontology/DedicatedSection
estat:DedicatedSection rdf:type owl:Class ;
                       rdfs:subClassOf estat:SEAReference ;
                       rdfs:comment "A class with the dedicated section resources" ;
                       rdfs:label "Dedicated Section" .


###  https://ec.europa.eu/eurostat/NLP4StatRef/ontology/EurostatTheme
estat:EurostatTheme rdf:type owl:Class ;
                    rdfs:subClassOf estat:Theme ;
                    rdfs:comment "A class with the Eurostat themes"^^xsd:string ;
                    rdfs:label "EurostatTheme"^^xsd:string .


###  https://ec.europa.eu/eurostat/NLP4StatRef/ontology/Excel
estat:Excel rdf:type owl:Class ;
            rdfs:subClassOf estat:SEAReference ;
            rdfs:comment "A class with references to excellence resources / articles / web sources" ;
            rdfs:label "Excel" .


###  https://ec.europa.eu/eurostat/NLP4StatRef/ontology/ExternalLink
estat:ExternalLink rdf:type owl:Class ;
                   rdfs:subClassOf estat:SEAReference ;
                   rdfs:comment "A class with the external references / articles / web sources" ;
                   rdfs:label "External Link" .


###  https://ec.europa.eu/eurostat/NLP4StatRef/ontology/FrequentTerm
estat:FrequentTerm rdf:type owl:Class ;
                   rdfs:subClassOf estat:GlossaryTerm ;
                   rdfs:comment "A class that contains the frequent terms discovered by Quantos in Euriostat's articles via PCA and topic modelling"^^xsd:string ;
                   rdfs:label "FrequentTerm"^^xsd:string .


###  https://ec.europa.eu/eurostat/NLP4StatRef/ontology/FurtherInfo
estat:FurtherInfo rdf:type owl:Class ;
                  rdfs:subClassOf estat:GAReference ;
                  rdfs:comment "A class with the further info references for the glossray articles" ;
                  rdfs:label "Further Info" .


###  https://ec.europa.eu/eurostat/NLP4StatRef/ontology/GAReference
estat:GAReference rdf:type owl:Class ;
                  rdfs:subClassOf estat:Reference ;
                  rdfs:comment "A class that contains all the subclass that indicate the type of references for the glossary articles" ;
                  rdfs:label "Glossary Articles References" .


###  https://ec.europa.eu/eurostat/NLP4StatRef/ontology/GlossaryArticle
estat:GlossaryArticle rdf:type owl:Class ;
                      rdfs:subClassOf estat:Article ;
                      rdfs:comment "A class with the Glossary Articles"^^xsd:string ;
                      rdfs:label "Glossary Article"^^xsd:string .


###  https://ec.europa.eu/eurostat/NLP4StatRef/ontology/GlossaryArticleCategory
estat:GlossaryArticleCategory rdf:type owl:Class ;
                              rdfs:subClassOf estat:Category ;
                              rdfs:comment "A class that contains the categories for the Glossary Articles"^^xsd:string ;
                              rdfs:label "GlossaryArticleCategory"^^xsd:string .


###  https://ec.europa.eu/eurostat/NLP4StatRef/ontology/GlossaryTerm
estat:GlossaryTerm rdf:type owl:Class ;
                   rdfs:comment "All types of controlled vocabularies, dictionaries, and others."@en ;
                   rdfs:label "GlossaryTerm"@en .


###  https://ec.europa.eu/eurostat/NLP4StatRef/ontology/InfoType
estat:InfoType rdf:type owl:Class ;
               rdfs:subClassOf estat:Type ;
               rdfs:comment "A class with the Information types"^^xsd:string ;
               rdfs:label "InfoType"^^xsd:string .


###  https://ec.europa.eu/eurostat/NLP4StatRef/ontology/Legislation
estat:Legislation rdf:type owl:Class ;
                  rdfs:subClassOf estat:SEAReference ;
                  rdfs:comment "A class with the legislation references / articles / web sources" ;
                  rdfs:label "Legislation" .


###  https://ec.europa.eu/eurostat/NLP4StatRef/ontology/LexicalType
estat:LexicalType rdf:type owl:Class ;
                  rdfs:subClassOf estat:Type ;
                  rdfs:comment "A class with the lexical types"^^xsd:string ;
                  rdfs:label "LexicalType"^^xsd:string .


###  https://ec.europa.eu/eurostat/NLP4StatRef/ontology/MeasurementType
estat:MeasurementType rdf:type owl:Class ;
                      rdfs:subClassOf estat:Type ;
                      rdfs:comment "A class with the measurement unit types"^^xsd:string ;
                      rdfs:label "MeasurementType"^^xsd:string .


###  https://ec.europa.eu/eurostat/NLP4StatRef/ontology/Methodology
estat:Methodology rdf:type owl:Class ;
                  rdfs:subClassOf estat:SEAReference ;
                  rdfs:comment "A class with the methodology references / articles / web sources" ;
                  rdfs:label "Methodology" .


###  https://ec.europa.eu/eurostat/NLP4StatRef/ontology/OECDTerm
estat:OECDTerm rdf:type owl:Class ;
               rdfs:subClassOf estat:GlossaryTerm ;
               rdfs:comment "A class that represents the OECD data" ;
               rdfs:label "OECDTerm" .


###  https://ec.europa.eu/eurostat/NLP4StatRef/ontology/OECDTheme
estat:OECDTheme rdf:type owl:Class ;
                rdfs:subClassOf estat:Theme ;
                rdfs:comment "A class that contains the OECD themes"^^xsd:string ;
                rdfs:label "OECDTheme"^^xsd:string .


###  https://ec.europa.eu/eurostat/NLP4StatRef/ontology/OtherArticle
estat:OtherArticle rdf:type owl:Class ;
                   rdfs:subClassOf estat:SEAReference ;
                   rdfs:comment "A class with other articles" ;
                   rdfs:label "Other Article" .


###  https://ec.europa.eu/eurostat/NLP4StatRef/ontology/Paragraph
estat:Paragraph rdf:type owl:Class ;
                rdfs:subClassOf estat:Content ;
                rdfs:comment "A class that contains the information for the paragraphs of the Statistics Explained Articles"^^xsd:string ;
                rdfs:label "Paragraph"^^xsd:string .


###  https://ec.europa.eu/eurostat/NLP4StatRef/ontology/Publication
estat:Publication rdf:type owl:Class ;
                  rdfs:subClassOf estat:SEAReference ;
                  rdfs:comment "A class with the publication references / articles / web sources" ;
                  rdfs:label "Publications" .


###  https://ec.europa.eu/eurostat/NLP4StatRef/ontology/Reference
estat:Reference rdf:type owl:Class ;
                rdfs:comment "A class that represents material (resources / articles / web sources) referenced from within an instance of class content (e.g. an article)"^^xsd:string ;
                rdfs:label "Reference"^^xsd:string .


###  https://ec.europa.eu/eurostat/NLP4StatRef/ontology/RelatedConcept
estat:RelatedConcept rdf:type owl:Class ;
                     rdfs:subClassOf estat:GAReference ;
                     rdfs:comment "A class with the related concepts references for the glossray articles" ;
                     rdfs:label "Related Concept" .


###  https://ec.europa.eu/eurostat/NLP4StatRef/ontology/RelatedStatisticalData
estat:RelatedStatisticalData rdf:type owl:Class ;
                             rdfs:subClassOf estat:GAReference ;
                             rdfs:comment "A class with the related statistical data references for the glossray articles" ;
                             rdfs:label "Related Staistical Data" .


###  https://ec.europa.eu/eurostat/NLP4StatRef/ontology/SEAReference
estat:SEAReference rdf:type owl:Class ;
                   rdfs:subClassOf estat:Reference ;
                   rdfs:comment "A class that contains all the subclass that indicate the type of references for the statistical explained articles" ;
                   rdfs:label "Statistics Explained Articles References" .


###  https://ec.europa.eu/eurostat/NLP4StatRef/ontology/Source
estat:Source rdf:type owl:Class ;
             rdfs:subClassOf estat:GAReference ;
             rdfs:comment "A class with the source references for the glossray articles" ;
             rdfs:label "Source" .


###  https://ec.europa.eu/eurostat/NLP4StatRef/ontology/StatisticalData
estat:StatisticalData rdf:type owl:Class ;
                      rdfs:subClassOf estat:Content ;
                      rdfs:comment "Abstract class for statistical content of the datasets"@en ;
                      rdfs:label "Statistical Data"@en .


###  https://ec.europa.eu/eurostat/NLP4StatRef/ontology/StatisticalType
estat:StatisticalType rdf:type owl:Class ;
                      rdfs:subClassOf estat:Type ;
                      rdfs:comment "A class with the statistical unit types"^^xsd:string ;
                      rdfs:label "StatisticalType"^^xsd:string .


###  https://ec.europa.eu/eurostat/NLP4StatRef/ontology/StatisticsExplainedArticle
estat:StatisticsExplainedArticle rdf:type owl:Class ;
                                 rdfs:subClassOf estat:Article ;
                                 rdfs:comment "A class with the statistics explained articles"^^xsd:string ;
                                 rdfs:label "StatisticsExplainedArticle"^^xsd:string .


###  https://ec.europa.eu/eurostat/NLP4StatRef/ontology/StatisticsExplainedCategory
estat:StatisticsExplainedCategory rdf:type owl:Class ;
                                  rdfs:subClassOf estat:Category ;
                                  rdfs:comment "A class that contains the categories for the Statistics Explained Articles"^^xsd:string ;
                                  rdfs:label "StatisticsExplainedCategory"^^xsd:string .


###  https://ec.europa.eu/eurostat/NLP4StatRef/ontology/StatusType
estat:StatusType rdf:type owl:Class ;
                 rdfs:subClassOf estat:Type ;
                 rdfs:comment "A class with the status types"^^xsd:string ;
                 rdfs:label "StatusType"^^xsd:string .


###  https://ec.europa.eu/eurostat/NLP4StatRef/ontology/Table
estat:Table rdf:type owl:Class ;
            rdfs:subClassOf estat:SEAReference ;
            rdfs:comment "A class with the resources of the tables" ;
            rdfs:label "Tables" .


###  https://ec.europa.eu/eurostat/NLP4StatRef/ontology/Theme
estat:Theme rdf:type owl:Class ;
            rdfs:subClassOf estat:Classification ;
            rdfs:comment "A class that represent the Themes that EuroStat offers"^^xsd:string ;
            rdfs:label "Theme"^^xsd:string .


###  https://ec.europa.eu/eurostat/NLP4StatRef/ontology/Topic
estat:Topic rdf:type owl:Class ;
            rdfs:subClassOf estat:Classification ;
            rdfs:comment "A class that represents the topics, given by the collegues at Quantos"^^xsd:string ;
            rdfs:label "Topic"^^xsd:string .


###  https://ec.europa.eu/eurostat/NLP4StatRef/ontology/Type
estat:Type rdf:type owl:Class ;
           rdfs:subClassOf estat:Classification ;
           rdfs:comment "A class that contains various types, statistical units, and measurement units among others"^^xsd:string ;
           rdfs:label "Type"^^xsd:string .


###  https://ec.europa.eu/eurostat/NLP4StatRef/ontology/Visualization
estat:Visualization rdf:type owl:Class ;
                    rdfs:subClassOf estat:SEAReference ;
                    rdfs:comment "A class with the visualization resources" ;
                    rdfs:label "Visualization" .


###  Generated by the OWL API (version 4.5.9.2019-02-01T07:24:44Z) https://github.com/owlcs/owlapi
